changed temp variables to use array instead of local
--HG--
branch : adt

platform/cito/CompileStmt.v
@@ -8,11 +8,9 @@ Section Compile.
 
   Variable layout : Layout.
 
-  Variable vars temp_vars : list string.
+  Variable vars : list string.
 
-  Require Import GoodVars.
-
-  Hypothesis h_good_vars : good_vars vars temp_vars.
+  Variable temp_size : nat.
 
   Variable imports : LabelMap.t assert.
 
@@ -29,9 +27,9 @@ Section Compile.
   Definition compile : cmd imports modName.
     refine (
         Wrap imports imports_global modName 
-             (CompileStmtImpl.compile layout vars temp_vars imports_global modName s k) 
-             (fun _ => postcond layout vars temp_vars k) 
-             (verifCond layout vars temp_vars s k) 
+             (CompileStmtImpl.compile layout vars temp_size imports_global modName s k) 
+             (fun _ => postcond layout vars temp_size k) 
+             (verifCond layout vars temp_size s k) 
              _ _).
     Require Import PostOk VerifCondOk.
     eapply post_ok.
