platform/cito/CompileStmtSpec.v
@@ -1,35 +1,35 @@
 Require Import Inv.
+Require Import Syntax.
 
 Set Implicit Arguments.
-
-Require Import ReservedNames.
-
-Require Import FreeVars.
-Require Import Depth.
-Require Import TempNames.
-Require Import StringSet.
-Require Import SetUtil.
-
-Definition in_scope vars temp_vars s := 
-  Subset (free_vars s) (to_set vars) /\
-  Subset (make_temp_names (depth s)) (to_set temp_vars).
-
-Require Import Syntax.
 
 Section Spec.
 
   Variable layout : Layout.
 
-  Variable vars temp_vars : list string.
+  Variable vars : list string.
+
+  Variable temp_size : nat.
 
   Variable s k : Stmt.
 
-  Definition precond := inv layout vars temp_vars (Seq s k).
+  Definition precond := inv layout vars temp_size (Seq s k).
 
-  Definition postcond := inv layout vars temp_vars k.
+  Definition postcond := inv layout vars temp_size k.
 
   Definition imply (pre new_pre: assert) := forall specs x, interp specs (pre x) -> interp specs (new_pre x).
 
-  Definition verifCond pre := imply pre precond :: in_scope vars temp_vars (Seq s k) :: nil.
+  Require Import FreeVars.
+  Require Import Depth.
+  Require Import StringSet.
+  Require Import SetUtil.
+
+  Local Open Scope nat.
+
+  Definition in_scope s := 
+    Subset (free_vars s) (to_set vars) /\
+    depth s <= temp_size.
+
+  Definition verifCond pre := imply pre precond :: in_scope (Seq s k) :: nil.
 
 End Spec.
