platform/cito/PostOk.v
@@ -8,11 +8,9 @@ Section TopSection.
 
   Variable layout : Layout.
 
-  Variable vars temp_vars : list string.
+  Variable vars : list string.
 
-  Require Import GoodVars.
-
-  Hypothesis h_good_vars : good_vars vars temp_vars.
+  Variable temp_size : nat.
 
   Variable imports : LabelMap.t assert.
 
@@ -29,12 +27,18 @@ Section TopSection.
   Lemma post_ok : 
     forall (pre : assert) (specs : codeSpec W (settings * state))
            (x : settings * state),
-      vcs (verifCond layout vars temp_vars s k pre) ->
+      vcs (verifCond layout vars temp_size s k pre) ->
       interp specs
              (Postcondition
-                (compile layout vars temp_vars imports_global modName s k pre) x) ->
-      interp specs (postcond layout vars temp_vars k x).
+                (compile layout vars temp_size imports_global modName s k pre) x) ->
+      interp specs (postcond layout vars temp_size k x).
   Proof.
+    (* unfold verifCond, imply; induction s. *)
+
+    (* (* skip *) *)
+    (* wrap0. *)
+    (* unfold_eval; repeat (first [do_wrap | do_unfold_eval | eval_step auto_ext]). *)
+    (* discharge_fs; descend; try clear_imports; repeat hiding ltac:(step auto_ext); eauto. *)
 
     admit.
   Qed.
