platform/cito/ReservedNames.v
@@ -1,9 +1,0 @@
-Require Import ShowNat.
-
-Set Implicit Arguments.
-
-Local Open Scope string_scope.
-
-Definition STACK_CAPACITY := "!reserved". 
-
-Definition temp_name := show_nat_unary "!".
