platform/cito/TempNames.v
@@ -1,9 +1,0 @@
-Require Import TempNamesList.
-Require Import StringSet.
-Require Import SetUtil.
-
-Set Implicit Arguments.
-
-Definition make_temp_names_range start len := to_set (make_temp_names_range_list start len).
-
-Definition make_temp_names := make_temp_names_range 0.
